scripts/hol-probes/regenerate.sh
@@ -582,7 +582,7 @@ run_probe crep_clock_leaf_eval_probeScript.sml crep_clock_leaf_eval_probe.out \
   if_true_eval if_false_eval if_error_eval if_nested_eval \
   seq_skip_break_eval seq_break_stops_eval seq_tick_skip_eval seq_tick_zero_eval \
   seq_fix_clock_upper_clamp_eval return_word_eval return_empty_eval \
-  return_missing_eval raise_eval \
+  return_missing_eval raise_eval dec_shadow_eval dec_new_local_eval dec_error_eval \
   "$cake_dir/pancake/semantics/crepSemScript.sml"
 run_probe pan_sem_call_return_shape_probeScript.sml pan_sem_call_return_shape_probe.out \
   call_bad_return_shape_result call_bad_return_shape_param_local \
